remake with both ocaml extraction + fun

harrison.v
@@ -1,8 +1,38 @@
 Require Import List.
+Import ListNotations.
 Require Import String.
+Require Import Lia.
+From Hammer Require Import Tactics.
+Require Import Coq.Program.Wf.
 
 Open Scope string_scope.
 Open Scope list_scope.
+
+(************)
+
+Program Fixpoint list_dec {A: Set} (l1: list A) (A_dec: forall a1, In a1 l1 -> forall a2, { a1 = a2 } + { a1 <> a2 }) (l2: list A) { struct l1 }: { l1 = l2 } + { l1 <> l2 } :=
+  match l1 with
+  | nil => _
+  | hd::tl => _ (@list_dec A tl _)
+  end.
+Next Obligation.
+  destruct l2; simpl; auto.
+  right; intro H; inversion H.
+Defined.
+Next Obligation.
+  destruct l2 ;simpl; auto.
+  right; intro H; inversion H.
+  assert (In hd (hd::tl)) by intuition.
+  generalize (A_dec _ H a); intro H1; inversion_clear H1.
+  subst a; generalize (x l2); intro H0; inversion_clear H0.
+  subst l2; left; intuition.
+  right; simpl; injection.
+  auto.
+  right; injection; intuition.
+Defined.
+Next Obligation.
+  intuition.
+Defined.
 
 (*****************************************)
 
@@ -13,20 +43,17 @@ Record InhabitedType : Type := {
 
 (*****************************************)
 
+(* term datatype + helper lemma/function *)
 
 Inductive term: Set :=
 | var: string -> term
 | fn: string -> list term -> term.
-
-(* now because we have list of term inside of term definition, we need to redefine our own induction scheme *)
 
 Fixpoint sum_list_nat (l: list nat) : nat :=
   match l with
   | nil => 0
   | hd::tl => hd + sum_list_nat tl
   end.
-
-Require Import Lia.
 
 Lemma sum_list_nat_elt: forall (l: list nat) (x: nat),
     In x l -> sum_list_nat l >= x.
@@ -53,17 +80,16 @@ generalize (IHl x H0); simpl; intros; auto.
 lia.
 Qed.
 
-Require Import Coq.Program.Wf.
-
 Program Fixpoint term_recursion
-        (P: term -> Type)
-        (P_var: forall s: string, P (var s))
-        (P_fn: forall (s: string) (l: list term),
-            (forall x, In x l -> P x) -> P (fn s l))
-        (t: term) { measure (term_measure t) } : P t :=
+  (t: term) 
+  (P: term -> Type)
+  (P_var: forall s: string, P (var s))
+  (P_fn: forall (s: string) (l: list term),
+      (forall x, In x l -> P x) -> P (fn s l))
+  { measure (term_measure t) } : P t :=
   match t with
   | var s => P_var s
-  | fn s l => P_fn s l (fun x H => term_recursion P P_var P_fn x)
+  | fn s l => P_fn s l (fun x H => term_recursion x P P_var P_fn)
   end.
 Next Obligation.  
 apply term_measure_elt; auto.
@@ -71,12 +97,12 @@ Qed.
 
 (* this is a couple simple rewriting rule that one could use for simplification in lemmas *)
 Lemma term_recursion_var P P_var P_fn: forall s,
-    term_recursion P P_var P_fn (var s) = P_var s.
+    term_recursion (var s) P P_var P_fn = P_var s.
 auto.
 Qed.
 
 Lemma term_recursion_fn P P_var P_fn: forall s l,
-    term_recursion P P_var P_fn (fn s l) = P_fn s l (fun x H => term_recursion P P_var P_fn x).
+    term_recursion (fn s l) P P_var P_fn = P_fn s l (fun x H => term_recursion x P P_var P_fn).
   intros.
   unfold term_recursion.
   unfold term_recursion_func.
@@ -100,7 +126,7 @@ Qed.
 
 (* specialization of the term_recursion rewriting rule *)
 Lemma term_recursion_map_term_var {A: Set} (f_var: string -> A) (f_fn: string -> list A -> A): forall s,
-    term_recursion (fun t => A) f_var (fun s l H => f_fn s (map_term l H)) (var s) =
+    term_recursion (var s) (fun t => A) f_var (fun s l H => f_fn s (map_term l H)) =
     f_var s.
   intros.
   rewrite term_recursion_var.
@@ -108,8 +134,8 @@ Lemma term_recursion_map_term_var {A: Set} (f_var: string -> A) (f_fn: string ->
 Qed.
   
   Lemma term_recursion_map_term_fn {A: Set} (f_var: string -> A) (f_fn: string -> list A -> A): forall s l,
-    term_recursion (fun t => A) f_var (fun s l H => f_fn s (map_term l H)) (fn s l) =
-    f_fn s (map (term_recursion (fun t => A) f_var (fun s l H => f_fn s (map_term l H))) l).
+    term_recursion (fn s l) (fun t => A) f_var (fun s l H => f_fn s (map_term l H)) =
+    f_fn s (map (fun t => term_recursion t (fun t => A) f_var (fun s l H => f_fn s (map_term l H))) l).
   intros.
   rewrite term_recursion_fn.
   f_equal.
@@ -119,35 +145,9 @@ Qed.
   rewrite <- IHl.
   auto.
 Qed.
-  
-(**)
-
-Program Fixpoint list_dec {A: Set} (l1: list A) (A_dec: forall a1, In a1 l1 -> forall a2, { a1 = a2 } + { a1 <> a2 }) (l2: list A) { struct l1 }: { l1 = l2 } + { l1 <> l2 } :=
-  match l1 with
-  | nil => _
-  | hd::tl => _ (@list_dec A tl _)
-  end.
-Next Obligation.
-  destruct l2; simpl; auto.
-  right; intro H; inversion H.
-Defined.
-Next Obligation.
-  destruct l2 ;simpl; auto.
-  right; intro H; inversion H.
-  assert (In hd (hd::tl)) by intuition.
-  generalize (A_dec _ H a); intro H1; inversion_clear H1.
-  subst a; generalize (x l2); intro H0; inversion_clear H0.
-  subst l2; left; intuition.
-  right; simpl; injection.
-  auto.
-  right; injection; intuition.
-Defined.
-Next Obligation.
-  intuition.
-Defined.
 
 Program Definition term_eq_dec (t1: term) : forall t2, { t1 = t2 } + { t1 <> t2 }:=
-  term_recursion (fun t => forall t2, { t = t2 } + { t <> t2 }) _ _ t1.
+  term_recursion t1 (fun t => forall t2, { t = t2 } + { t <> t2 }) _ _.
 Next Obligation.
   destruct t2.
   generalize (string_dec s s0); intro H0; inversion_clear H0.
@@ -165,41 +165,8 @@ Next Obligation.
   right; injection; intuition.
 Defined.
 
-(**)
-
-
-Definition term_semantics
-           {Value: InhabitedType}
-           (ctxt_var: string -> Value)
-           (ctxt_fn: string -> list Value -> Value)
-           (t: term): Value :=
-  term_recursion (fun t => Value) ctxt_var (fun s l H => ctxt_fn s (map_term l H)) t.
-
-Lemma term_semantics_var
-      {Value: InhabitedType}
-      (ctxt_var: string -> Value)
-      (ctxt_fn: string -> list Value -> Value): forall s,
-    term_semantics ctxt_var ctxt_fn (var s) =
-    ctxt_var s.
-  intros.
-  unfold term_semantics.
-  apply term_recursion_map_term_var.
-Qed.
-
-
-Lemma term_semantics_fn
-      {Value: InhabitedType}
-      (ctxt_var: string -> Value)
-      (ctxt_fn: string -> list Value -> Value): forall s l,
-    term_semantics ctxt_var ctxt_fn (fn s l) =
-    ctxt_fn s (map (term_semantics ctxt_var ctxt_fn) l).
-  intros.
-  unfold term_semantics.
-  apply term_recursion_map_term_fn.
-Qed.
-
 Definition term_free_vars (t: term): list string :=
-  term_recursion (fun t => list string) (fun s => s::nil) (fun s l H => List.concat (map_term l H)) t.
+  term_recursion t (fun t => list string) (fun s => s::nil) (fun s l H => List.concat (map_term l H)).
 
 Lemma term_free_vars_fn: forall s l,
     term_free_vars (fn s l) = List.concat (map term_free_vars l).
@@ -208,42 +175,12 @@ Lemma term_free_vars_fn: forall s l,
   apply term_recursion_map_term_fn with (f_fn := fun s l => List.concat l).
 Qed.
 
-Program Definition term_semantics_free_vars
-        {Value: InhabitedType}
-        (t: term)
-        (ctxt_fn: string -> list Value -> Value)
-        (ctxt_var1: string -> Value)
-        (ctxt_var2: string -> Value):
-        (forall s, List.In s (term_free_vars t) -> ctxt_var1 s = ctxt_var2 s) ->
-  @term_semantics Value ctxt_var1 ctxt_fn t = @term_semantics Value ctxt_var2 ctxt_fn t :=
-  term_recursion (fun t =>
-                    (forall s, List.In s (term_free_vars t) -> ctxt_var1 s = ctxt_var2 s) ->
-                    @term_semantics Value ctxt_var1 ctxt_fn t = @term_semantics Value ctxt_var2 ctxt_fn t) _ _ t.
-Next Obligation.
-cut (ctxt_var1 s = ctxt_var2 s); intuition.
-Qed.
-Next Obligation.
-  do 2 rewrite term_semantics_fn.
-  f_equal.
-  apply map_ext_in; intros.
-  apply H; auto.
-  intros.
-  apply H0.
-  rewrite term_free_vars_fn.
-  rewrite <- flat_map_concat_map; rewrite in_flat_map; exists a; auto.
-Qed.
-  
-(*****************************************)
+(**************************************)
 
-(* this is just really to match the ocaml code on extraction *)
-
-Inductive fol: Set :=
-  | R: string -> list term -> fol.
-
-Inductive formula {A: Set}: Set :=
-| True: formula
-| False: formula
-| Atom: A -> formula
+Inductive formula: Set :=
+| true: formula
+| false: formula
+| Atom: string -> list term -> formula
 | Eq: term -> term -> formula
 | Not: formula -> formula
 | And: formula -> formula -> formula
@@ -251,12 +188,18 @@ Inductive formula {A: Set}: Set :=
 | Imp: formula -> formula -> formula
 | Iff: formula -> formula -> formula
 | Forall: string -> formula -> formula
-| Exists: string -> formula -> formula
-.
+| Exists: string -> formula -> formula.
 
+Notation "x1 == x2" := (Eq x1 x2) (at level 70, right associativity).
+Notation "~~ b" := (Not b) (at level 75, right associativity).
+Notation "b1 //\\ b2" := (And b1 b2) (at level 80, right associativity).
+Notation "b1 \\// b2" := (Or b1 b2) (at level 85, right associativity).
+Notation "b1 ==> b2" := (Imp b1 b2) (at level 90, right associativity).
+Notation "b1 <=> b2" := (Iff b1 b2) (at level 90, right associativity).
+Notation "'F' x , f" := (Forall x f) (at level 100, right associativity).
+Notation "'E' x , f" := (Exists x f) (at level 100, right associativity).
 
-Definition formula_dec: forall (f1 f2: @formula fol), {f1 = f2} + {f1 <> f2}.
-  decide equality.
+Definition formula_dec: forall (f1 f2: formula), {f1 = f2} + {f1 <> f2}.
   decide equality.
   apply List.list_eq_dec; apply term_eq_dec.
   apply string_dec.
@@ -266,45 +209,126 @@ Definition formula_dec: forall (f1 f2: @formula fol), {f1 = f2} + {f1 <> f2}.
   apply string_dec.
 Defined.
 
-Fixpoint formula_semantics 
-         {Value: InhabitedType}
-         (ctxt_var: string -> Value)
-         (ctxt_fn: string -> list Value -> Value)
-         (ctxt_pred: string -> list Value -> Prop)
-         (f: @formula fol) : Prop :=
+(***************************************)
+
+Record Model {Value: InhabitedType}: Type := {
+    var_sem: string -> Value;
+    fn_sem: string -> list Value -> Value;
+    pred_sem: string -> list Value -> Prop;
+  }.
+
+Definition eval {V} (m: @Model V) (t: term) : V :=
+  term_recursion t (fun _ => V) (var_sem m) (fun s l H => (fn_sem m) s (map_term l H)).
+
+Lemma eval_var {V} (m: @Model V):
+  forall s,
+    eval m (var s) = var_sem m s. 
+sauto.
+Qed.
+
+Lemma eval_fn {V} (m: @Model V):
+  forall f l,
+    eval m (fn f l) = fn_sem m f (map (eval m) l).
+  intros.
+  unfold eval.
+  apply term_recursion_map_term_fn.
+Qed.
+
+Lemma free_vars_term_sem {V}:
+  forall (t: term) (m1 m2: @Model V),
+    (forall s, List.In s (term_free_vars t) -> var_sem m1 s = var_sem m2 s) ->
+    (forall f l, fn_sem m1 f l = fn_sem m2 f l) ->
+    eval m1 t = eval m2 t.
+  intro.
+  apply (term_recursion t); simpl; intros.
+  do 2 rewrite eval_var.
+  sauto.
+  do 2 rewrite eval_fn.
+  rewrite H1.
+  f_equal.
+  apply map_ext_in; intros.
+  apply H; auto; intros.
+  apply H0.
+  rewrite term_free_vars_fn.
+  rewrite <- flat_map_concat_map; rewrite in_flat_map; exists a; auto.
+Qed.
+
+Lemma free_vars_terms_sem {V}:
+  forall (l: list term) (m1 m2: @Model V),
+    (forall s, List.In s (List.concat (map term_free_vars l)) -> var_sem m1 s = var_sem m2 s) ->
+    (forall f l, fn_sem m1 f l = fn_sem m2 f l) ->
+    map (eval m1) l = map (eval m2) l.
+  induction l; simpl; intros; auto.
+  rewrite (free_vars_term_sem a m1 m2); auto.
+  rewrite (IHl m1 m2); auto.
+  intros; apply H; intuition.
+  intros; apply H; intuition.
+Qed.
+
+Definition updated_model {V} (m: @Model V) (x: string) (v: V): @Model V :=
+  {| var_sem := fun s => match string_dec x s with | left _ => v | right _ => var_sem m s end ;
+    fn_sem := fn_sem m;
+    pred_sem := pred_sem m ;
+  |}.
+
+Lemma updated_model_var_sem1 {V} (m: @Model V) (x: string) (v: V):
+  forall y, x <> y -> var_sem (updated_model m x v) y = var_sem m y.
+  destruct m.
+  simpl; intros.
+  sauto.
+Qed.
+
+Lemma updated_model_var_sem2 {V} (m: @Model V) (x: string) (v: V):
+  forall y, x = y -> var_sem (updated_model m x v) y = v.
+  destruct m.
+  simpl; intros.
+  sauto.
+Qed.
+
+Lemma updated_model_fn_sem {V} (m: @Model V) (x: string) (v: V):
+  forall f l,
+    fn_sem m f l = fn_sem (updated_model m x v) f l.
+  destruct m.
+  simpl; intros.
+  sauto.
+Qed.
+
+Lemma updated_model_pred_sem {V} (m: @Model V) (x: string) (v: V):
+  forall p l,
+    pred_sem m p l <-> pred_sem (updated_model m x v) p l.
+  destruct m.
+  simpl; intros.
+  sauto.
+Qed.
+
+Fixpoint models {V} (m: @Model V) (f: formula): Prop :=
   match f with
-  | True => Logic.True
-  | False => Logic.False
-  | Atom (R P args) => ctxt_pred P (map (term_semantics ctxt_var ctxt_fn) args)
-  | Eq t1 t2 => term_semantics ctxt_var ctxt_fn t1 = term_semantics ctxt_var ctxt_fn t2
-  | Not f => ~ (formula_semantics ctxt_var ctxt_fn ctxt_pred f)
-  | And f1 f2 => (formula_semantics ctxt_var ctxt_fn ctxt_pred f1) /\ (formula_semantics ctxt_var ctxt_fn ctxt_pred f2) 
-  | Or f1 f2 => (formula_semantics ctxt_var ctxt_fn ctxt_pred f1) \/ (formula_semantics ctxt_var ctxt_fn ctxt_pred f2) 
-  | Imp f1 f2 => (formula_semantics ctxt_var ctxt_fn ctxt_pred f1) -> (formula_semantics ctxt_var ctxt_fn ctxt_pred f2) 
-  | Iff f1 f2 => (formula_semantics ctxt_var ctxt_fn ctxt_pred f1) <-> (formula_semantics ctxt_var ctxt_fn ctxt_pred f2)
-  | Forall x f => forall (v: Value),
-      formula_semantics
-        (fun y => match string_dec x y with | left _ => v | right _ => ctxt_var y end)
-        ctxt_fn ctxt_pred f
-  | Exists x f => exists (v: Value),
-      formula_semantics
-        (fun y => match string_dec x y with | left _ => v | right _ => ctxt_var y end)
-        ctxt_fn ctxt_pred f
+  | true => True
+  | false => False
+  | Atom P args => pred_sem m P (map (eval m) args)
+  | Eq t1 t2 => eval m t1 = eval m t2
+  | Not f => ~ models m f
+  | And f1 f2 => models m f1 /\ models m f2
+  | Or f1 f2 => models m f1 \/ models m f2
+  | Imp f1 f2 => models m f1 -> models m f2
+  | Iff f1 f2 => models m f1 <-> models m f2
+  | Forall x f => forall v: V,
+      models (updated_model m x v) f
+  | Exists x f => exists v: V,
+      models (updated_model m x v) f
   end.
 
-Axiom classical_formula:
-  forall {Value: InhabitedType}
-         (ctxt_var: string -> Value)
-         (ctxt_fn: string -> list Value -> Value)
-         (ctxt_pred: string -> list Value -> Prop)
-         (f: formula),
-    (formula_semantics ctxt_var ctxt_fn ctxt_pred f) \/ ~ (formula_semantics ctxt_var ctxt_fn ctxt_pred f).
+Notation "m '|=' f" := (@models _ m f) (at level 150, right associativity).
+
+Axiom models_classical:
+  forall {V} (m: @Model V) (f: formula),
+    (m |= f) \/ ~ (m |= f).
 
 Fixpoint formula_free_vars (f: formula) : list string :=
     match f with
-  | True => nil
-  | False => nil
-  | Atom (R P args) => List.concat (map term_free_vars args)
+  | true => nil
+  | false => nil
+  | Atom P args => List.concat (map term_free_vars args)
   | Eq t1 t2 => term_free_vars t1 ++ term_free_vars t2
   | Not f => formula_free_vars f
   | And f1 f2 => formula_free_vars f1 ++ formula_free_vars f2
@@ -314,7 +338,7 @@ Fixpoint formula_free_vars (f: formula) : list string :=
   | Forall x f => List.remove string_dec x (formula_free_vars f)
   | Exists x f => List.remove string_dec x (formula_free_vars f)
   end.
-  
+
 Lemma remove_In_diff: forall {A: Set} H
                              (l: list A) (x x0: A), x <> x0 -> List.In x l -> List.In x (@List.remove _ H x0 l).
   do 2 intro.
@@ -325,108 +349,505 @@ Lemma remove_In_diff: forall {A: Set} H
   destruct (H x0 a); intuition.
 Qed.
 
-Lemma formula_semantics_free_vars:
-  forall
-      {Value: InhabitedType}
-      (f: formula)
-      (ctxt_fn: string -> list Value -> Value)
-      (ctxt_pred: string -> list Value -> Prop)
-      (ctxt_var1: string -> Value)
-      (ctxt_var2: string -> Value)
-      (Hyp: forall s, List.In s (formula_free_vars f) -> ctxt_var1 s = ctxt_var2 s),
-  (formula_semantics ctxt_var1 ctxt_fn ctxt_pred f) <-> (formula_semantics ctxt_var2 ctxt_fn ctxt_pred f).
+Lemma formula_vars_term_sem {V}:
+  forall (f: formula) (m1 m2: @Model V),
+    (forall s, List.In s (formula_free_vars f) -> var_sem m1 s = var_sem m2 s) ->
+    (forall f l, fn_sem m1 f l = fn_sem m2 f l) ->
+    (forall p l, pred_sem m1 p l = pred_sem m2 p l) ->
+    (m1 |= f) <-> (m2 |= f).
+induction f; simpl; intros; auto.
 
-  induction f; simpl; intros.
+intuition.
 
-  intuition.
-  intuition.
+intuition.
 
-  destruct a.
-  cut (map (term_semantics ctxt_var1 ctxt_fn) l = map (term_semantics ctxt_var2 ctxt_fn) l).
-  intro H; rewrite H; split; auto.
-  apply map_ext_in; intros.
-  eapply term_semantics_free_vars.
-  intuition.
-  eapply Hyp.
-  rewrite <- flat_map_concat_map; rewrite in_flat_map; exists a; auto.
+rewrite <- H1.
+rewrite (free_vars_terms_sem l m1 m2); auto.
+intuition.
+rewrite (free_vars_term_sem t m2 m1); auto.
+rewrite (free_vars_term_sem t0 m2 m1); auto.
+intuition.  
+intros; rewrite H; intuition.
+intros; rewrite H; intuition.
 
-  rewrite term_semantics_free_vars with (ctxt_var1 := ctxt_var1) (ctxt_var2 := ctxt_var2).
-  rewrite term_semantics_free_vars with (ctxt_var1 := ctxt_var1) (ctxt_var2 := ctxt_var2).
-  intuition.
-  intros; apply Hyp; apply List.in_or_app; right; auto.
-  intros; apply Hyp; apply List.in_or_app; left; auto.
+rewrite IHf; auto.
+intuition.
 
-  rewrite IHf with (ctxt_var1 := ctxt_var1) (ctxt_var2 := ctxt_var2); intuition.
+rewrite (IHf1 m1 m2); auto.
+rewrite (IHf2 m1 m2); auto.
+intuition.
+intros; apply H; intuition.
+intros; apply H; intuition.
 
-  rewrite IHf1 with (ctxt_var1 := ctxt_var1) (ctxt_var2 := ctxt_var2).
-  rewrite IHf2 with (ctxt_var1 := ctxt_var1) (ctxt_var2 := ctxt_var2).
-  intuition.
-  intuition.
-  intuition.
+rewrite (IHf1 m1 m2); auto.
+rewrite (IHf2 m1 m2); auto.
+intuition.
+intros; apply H; intuition.
+intros; apply H; intuition.
 
-  rewrite IHf1 with (ctxt_var1 := ctxt_var1) (ctxt_var2 := ctxt_var2).
-  rewrite IHf2 with (ctxt_var1 := ctxt_var1) (ctxt_var2 := ctxt_var2).
-  intuition.
-  intuition.
-  intuition.
+rewrite (IHf1 m1 m2); auto.
+rewrite (IHf2 m1 m2); auto.
+intuition.
+intros; apply H; intuition.
+intros; apply H; intuition.
 
-  rewrite IHf1 with (ctxt_var1 := ctxt_var1) (ctxt_var2 := ctxt_var2).
-  rewrite IHf2 with (ctxt_var1 := ctxt_var1) (ctxt_var2 := ctxt_var2).
-  intuition.
-  intuition.
-  intuition.
+rewrite (IHf1 m1 m2); auto.
+rewrite (IHf2 m1 m2); auto.
+intuition.
+intros; apply H; intuition.
+intros; apply H; intuition.
 
-  rewrite IHf1 with (ctxt_var1 := ctxt_var1) (ctxt_var2 := ctxt_var2).
-  rewrite IHf2 with (ctxt_var1 := ctxt_var1) (ctxt_var2 := ctxt_var2).
-  intuition.
-  intuition.
-  intuition.
+split; intros; auto.
+(**)
+rewrite <- (IHf (updated_model m1 s v) (updated_model m2 s v)); auto.
+intros.
+destruct (string_dec s s0); auto.
+rewrite (updated_model_var_sem2 m1 s v); auto.
+rewrite (updated_model_var_sem2 m2 s v); auto.
+rewrite (updated_model_var_sem1 m1 s v); auto.
+rewrite (updated_model_var_sem1 m2 s v); auto.
+apply H; auto.
+apply remove_In_diff; auto.
+(**)
+rewrite (IHf (updated_model m1 s v) (updated_model m2 s v)); auto.
+intros.
+destruct (string_dec s s0); auto.
+rewrite (updated_model_var_sem2 m1 s v); auto.
+rewrite (updated_model_var_sem2 m2 s v); auto.
+rewrite (updated_model_var_sem1 m1 s v); auto.
+rewrite (updated_model_var_sem1 m2 s v); auto.
+apply H; auto.
+apply remove_In_diff; auto.
 
-  split; intros; intuition.
-  rewrite IHf with (ctxt_var2 := (fun y : string => if string_dec s y then v else ctxt_var1 y)); auto.
-  intros.
-  destruct (string_dec s s0); auto.
-  rewrite Hyp; auto.
-  apply remove_In_diff; intuition.
+split; intros; auto.
+(**)
+inversion_clear H2.
+exists x.
+rewrite <- (IHf (updated_model m1 s x) (updated_model m2 s x)); auto.
+intros.
+destruct (string_dec s s0); auto.
+rewrite (updated_model_var_sem2 m1 s x); auto.
+rewrite (updated_model_var_sem2 m2 s x); auto.
+rewrite (updated_model_var_sem1 m1 s x); auto.
+rewrite (updated_model_var_sem1 m2 s x); auto.
+apply H; auto.
+apply remove_In_diff; auto.
+(**)
+inversion_clear H2.
+exists x.
+rewrite (IHf (updated_model m1 s x) (updated_model m2 s x)); auto.
+intros.
+destruct (string_dec s s0); auto.
+rewrite (updated_model_var_sem2 m1 s x); auto.
+rewrite (updated_model_var_sem2 m2 s x); auto.
+rewrite (updated_model_var_sem1 m1 s x); auto.
+rewrite (updated_model_var_sem1 m2 s x); auto.
+apply H; auto.
+apply remove_In_diff; auto.
 
-  rewrite IHf with (ctxt_var2 := (fun y : string => if string_dec s y then v else ctxt_var2 y)); auto.
-  intros.
-  destruct (string_dec s s0); auto.
-  rewrite Hyp; auto.
-  apply remove_In_diff; intuition.
-
-  split; intros; intuition.
-  inversion_clear H.
-  exists x.
-  rewrite IHf with (ctxt_var2 := (fun y : string => if string_dec s y then x else ctxt_var1 y)); auto.
-  intros.
-  destruct (string_dec s s0); auto.
-  rewrite Hyp; auto.
-  apply remove_In_diff; intuition.
-  inversion_clear H.
-  exists x.
-  rewrite IHf with (ctxt_var2 := (fun y : string => if string_dec s y then x else ctxt_var2 y)); auto.
-  intros.
-  destruct (string_dec s s0); auto.
-  rewrite Hyp; auto.
-  apply remove_In_diff; intuition.
 Qed.
 
-(*****************************************)
+
+Definition is_valid (f: formula) : Prop :=
+  forall {V} (m: @Model V),
+    m |= f.
+
+Notation "'|-' f" := (is_valid f) (at level 150, right associativity).
+
+Lemma modusponens {p q: formula}:
+  forall (A: |- p ==> q)
+         (B: |- p),
+    (|- q).
+  unfold is_valid.
+  intros.
+  generalize (A V m); clear A; intro A.
+  generalize (B V m); clear B; intro B.
+  apply A.
+  auto.
+Qed.
+
+Lemma lemma_gen {p: formula}:
+  forall (H: |- p) x,
+    (|- Forall x p).
+  unfold is_valid.
+  intros.
+  simpl; intros.
+  apply H.
+Qed.
+
+Lemma lemma_addimp (p q: formula):
+  |- p ==> (q ==> p).
+  red.
+  intros.
+  intro.
+  intro.
+  auto.
+Qed.
+
+Lemma lemma_distribimp (p q r: formula):
+      |- (p ==> q ==> r) ==> (p ==> q) ==> (p ==> r).
+  red; intros.
+  intro.
+  intro.
+  intro.
+  apply H.
+  apply H1.
+  apply H0.
+  apply H1.
+Qed.
+
+Lemma lemma_doubleneg (p : formula):
+      |- ((p ==> false) ==> false) ==> p.
+  red; intros.
+  intro.
+  destruct (models_classical m p); auto.
+  generalize (H H0); intros; intuition.
+Qed.
+
+Lemma lemma_allimp x (p q: formula) :
+  |- (F x, p ==> q) ==> (F x, p) ==> (F x, q).
+  red; intros.
+  intro.
+  intro.
+  intro.
+  apply H.
+  apply H0.
+Qed.
+
+Lemma lemma_impall x (p: formula):
+  ~ In x (formula_free_vars p) ->
+  |- p ==> Forall x p.
+  intros.
+  red; intros.
+  intro.
+  intro.
+  rewrite (formula_vars_term_sem _ _ m); auto.
+  intros; auto.
+  destruct (string_dec x s); auto.
+  subst x; intuition.
+  rewrite updated_model_var_sem1; auto.
+Qed.
+
+Lemma lemma_existseq x (t: term):
+  ~ In x (term_free_vars t) ->
+      |- Exists x (var x == t).
+  red; intros.
+  exists (eval m t).
+  simpl.
+  rewrite eval_var.
+  rewrite updated_model_var_sem2; auto.  
+  rewrite (free_vars_term_sem t (updated_model m x (eval m t)) m); auto; intros.
+  rewrite updated_model_var_sem1; auto.  
+  intro; subst x; intuition.
+Qed.
+
+Lemma lemma_eqrefl (t: term):
+  |- t == t.
+  red; intros.
+  red; auto.
+Qed.
+
+Lemma lemma_iffimp1 (p q: formula):
+      |- (p <=> q) ==> p ==> q.
+  red; intros.
+  intro.
+  inversion_clear H.  
+  intuition.
+Qed.
+
+Lemma lemma_iffimp2 (p q: formula):
+      |- (p <=> q) ==> q ==> p.
+  red; intros.
+  intro.
+  inversion_clear H.  
+  intuition.
+Qed.
+
+Lemma lemma_impiff (p q: formula):
+      |- (p ==> q) ==> (q ==> p) ==> (p <=> q).
+  red; intros.
+  intro.
+  intro.
+  split; intuition.
+Qed.  
+
+Lemma lemma_true:
+      |- true <=> (false ==> false).
+  red; intros.
+  split; intro.
+  intro; intuition.
+  red; auto.
+Qed.
+
+Lemma lemma_not (p: formula):
+      |- ~~ p <=> (p ==> false) .
+  red; intros.
+  split; intros; intuition.
+Qed.
+
+Lemma lemma_and (p q: formula):
+      |- p //\\ q <=> (p ==> q ==> false) ==> false.
+  red; intros.
+  split; intuition.
+  inversion_clear H.
+  intro.
+  apply H; intuition.
+  destruct (models_classical m (p //\\ q)); intuition.
+  assert False; intuition.
+  apply H.
+  intros.
+  apply H0.
+  split; intuition.
+Qed.
+  
+Lemma lemma_or (p q: formula):
+      |- p \\// q <=> ~~(~~ p //\\ ~~ q).
+  split; intros.
+  intro.
+  inversion_clear H0.
+  inversion_clear H; intuition.
+  destruct (models_classical m (p \\// q)); intuition.
+  assert False; intuition.
+  apply H.
+  split; intro; apply H0.
+  left; intuition.
+  right; intuition.
+Qed.  
+
+Lemma lemma_exists x (p: formula):
+      |- (E x, p) <=> ~~(F x, ~~p).
+  red; intros.
+  split; intro.
+  intro.
+  inversion_clear H.
+  apply (H0 x0).
+  sauto.
+  destruct (models_classical m (E x, p)); intuition.
+  cut False; intuition.
+  apply H.
+  sauto.
+Qed.
+
+(* need to cleanup *)
+
+Fixpoint unzip (l: list (term * term)): list term * list term :=
+  match l with
+  | nil => (nil, nil)
+  | (hd1, hd2)::tl =>
+      let (tl1, tl2) := unzip tl in
+      (hd1::tl1, hd2::tl2)
+  end.
+
+Lemma unzip_fst_snd: forall l,
+    unzip l = (fst (unzip l), snd (unzip l)).
+  induction l; simpl; intros; auto.
+  rewrite IHl; simpl.
+  destruct a; simpl; auto.
+Qed.  
+  
+Lemma unzip_unfold: forall tl hd1 hd2,
+    unzip ((hd1, hd2)::tl) = (hd1::(fst (unzip tl)), hd2::(snd (unzip tl))).
+  induction tl.
+  intuition.
+  intros.
+  destruct a.
+  rewrite (IHtl t t0).
+  sauto.
+Qed.
+  
+Lemma l1 (l: list( term * term)) {V} (m: @Model V):
+    (forall x, In x l -> let (x1, x2) := x in eval m x1 = eval m x2) ->
+    let (l1, l2) := unzip l in
+    map (eval m) l1 = map (eval m) l2.
+  induction l; simpl; intros; auto.
+  destruct a.
+  rewrite unzip_fst_snd.
+  simpl.
+  rewrite (H (t, t0)); intuition.
+  cutrewrite (map (eval m) (fst (unzip l)) =
+                map (eval m) (snd (unzip l))
+             ); intuition.
+  rewrite unzip_fst_snd in IHl.
+  rewrite IHl; intuition.
+  apply H; intuition.
+Qed.
+
+Lemma l1_2 (l: list( term * term)) {V} (m: @Model V):
+    (forall x, In x l -> let (x1, x2) := x in eval m x1 = eval m x2) ->    
+    map (eval m) (fst (unzip l)) = map (eval m) (snd (unzip l)).
+  intros.
+  generalize (l1 _ _ H); intros.
+  rewrite unzip_fst_snd in H0; intuition.
+Qed.  
+
+Lemma l2 (l: list( term * term)) {V} (m: @Model V) f:
+  (forall x, In x l -> let (x1, x2) := x in eval m x1 = eval m x2) ->
+  let (l1, l2) := unzip l in
+  m |= fn f l1 == fn f l2.  
+  intros.
+  rewrite unzip_fst_snd.
+  red.
+  do 2 rewrite eval_fn.
+  rewrite l1_2; intuition.
+Qed.
+
+Lemma eq_fun (l: list( term * term)) {V} (m: @Model V) f:
+  (forall x, In x l -> let (x1, x2) := x in eval m x1 = eval m x2) ->
+  let (l1, l2) := unzip l in
+  m |= fn f l1 == fn f l2.  
+  intros.
+  rewrite unzip_fst_snd.
+  red.
+  do 2 rewrite eval_fn.
+  rewrite l1_2; intuition.
+Qed.
+
+Lemma eq_pred (l: list( term * term)) {V} (m: @Model V) P:
+  (forall x, In x l -> let (x1, x2) := x in eval m x1 = eval m x2) ->
+  let (l1, l2) := unzip l in
+  m |= Atom P l1 ==> Atom P l2.  
+  intros.
+  rewrite unzip_fst_snd.
+  red.
+  rewrite l1_2; intuition.
+Qed.
+
+Fixpoint formulas_conj (l: list formula) : formula :=
+  match l with
+  | nil => true
+  | hd::tl => hd //\\ formulas_conj tl
+  end.
+
+Lemma conj_forall_eq_m (l: list formula) {V} (m: @Model V):
+  (forall x, In x l -> m |= x) <->
+    (m |= formulas_conj l).
+  induction l; simpl; intros.
+  split; intros; intuition.
+  sauto.
+Qed.
+
+Lemma conj_forall_eq_v (l: list formula) {V} (m: @Model V):
+  (forall x, In x l -> |- x) <->
+    (|- formulas_conj l).
+  induction l; simpl; intros.
+  split; intros; sauto.  
+  split; simpl; intros; auto.
+  generalize (H a); intros; sauto.
+  inversion_clear H0.  
+  subst x; red; intros.
+  generalize (H _ m0); intro H1; inversion_clear H1; auto.
+  inversion_clear IHl.
+  apply H2; auto.
+  red; intros.
+  generalize (H _ m0); intros; sauto.
+Qed.
+
+Lemma conj_forall_eq (l: list (term * term)) {V} (m: @Model V):
+  (forall x, In x l -> let (x1, x2) := x in eval m x1 = eval m x2) <->
+    (m |= formulas_conj (map (fun x => fst x == snd x) l)).
+  induction l; simpl; intros; auto.
+  sauto.
+  split; simpl; intros; auto.
+  sauto.
+  sauto.
+Qed.
+  
+Fixpoint formulas_imp (l: list formula) (ccl: formula): formula :=
+  match l with
+  | nil => ccl
+  | hd::tl => hd ==> formulas_imp tl ccl
+  end.
+
+Lemma build_conj_imp_equiv {V} (m: @Model V) (l: list formula) (ccl: formula):
+  (m |= formulas_conj l ==> ccl) <-> (m |= formulas_imp l ccl).
+  induction l; simpl; intros; auto.  
+  sauto.
+  rewrite <- IHl.
+  sauto.
+Qed.  
+(*
+Lemma build_conj_imp_equiv {V} (m: @Model V) (l: list (term * term)) (ccl: formula):
+  (m |= (formulas_conj (map (fun x => fst x == snd x) l)) ==> ccl) <-> (m |= formulas_imp (map (fun x => fst x == snd x) l) ccl).
+  induction l; simpl; intros; auto.  
+  sauto.
+  rewrite <- IHl.
+  sauto.
+Qed.  
+ *)
+
+Lemma lemma_fun_congruence_aux f (l: list (term * term)):
+  let (l1, l2) := unzip l in
+  |- formulas_imp (map (fun x => fst x == snd x) l) (fn f l1 == fn f l2).
+  rewrite unzip_fst_snd.
+  red; intros.
+  rewrite <- build_conj_imp_equiv.
+  intro.
+  generalize (conj_forall_eq l m); intros.
+  generalize (eq_fun l m f); intros.
+  rewrite unzip_fst_snd in H1.
+  apply H1.
+  sauto.
+Qed.
+
+Lemma lemma_funcong_ f (l: list (term * term)):
+  let (l1, l2) := unzip l in
+  |- formulas_imp (map (fun x => fst x == snd x) l) (fn f l1 == fn f l2).
+  rewrite unzip_fst_snd.
+  red; intros.
+  rewrite <- build_conj_imp_equiv.
+  intro.
+  generalize (conj_forall_eq l m); intros.
+  generalize (eq_fun l m f); intros.
+  rewrite unzip_fst_snd in H1.
+  apply H1.
+  sauto.
+Qed.
+
+Lemma lemma_funcong f (l: list (term * term)):
+      |- formulas_imp (map (fun x => fst x == snd x) l) (fn f (fst (unzip l)) == fn f (snd (unzip l))).
+  red; intros.
+  rewrite <- build_conj_imp_equiv.
+  intro.
+  generalize (conj_forall_eq l m); intros.
+  generalize (eq_fun l m f); intros.
+  rewrite unzip_fst_snd in H1.
+  apply H1.
+  sauto.
+Qed.
+
+Lemma lemma_predcong_ P (l: list (term * term)):
+  let (l1, l2) := unzip l in
+  |- formulas_imp (map (fun x => fst x == snd x) l) (Atom P l1 ==> Atom P l2).
+  rewrite unzip_fst_snd.
+  red; intros.
+  rewrite <- build_conj_imp_equiv.
+  intro.
+  generalize (conj_forall_eq l m); intros.
+  generalize (eq_pred l m P); intros.
+  rewrite unzip_fst_snd in H1.
+  apply H1.
+  sauto.
+Qed.
+
+Lemma lemma_predcong P (l: list (term * term)):
+  |- formulas_imp (map (fun x => fst x == snd x) l) (Atom P (fst (unzip l)) ==> Atom P (snd (unzip l))).
+  red; intros.
+  rewrite <- build_conj_imp_equiv.
+  intro.
+  generalize (conj_forall_eq l m); intros.
+  generalize (eq_pred l m P); intros.
+  rewrite unzip_fst_snd in H1.
+  apply H1.
+  sauto.
+Qed.
+
+(*** Module for Ocaml extraction  ***)
 
 Module Type ProofSystem.
 
   Parameter Thm: Set.
-  Parameter concl: Thm -> @formula fol.
-
-  Parameter proof:
-    forall (thm: Thm)
-           {Value: InhabitedType}
-           (ctxt_var: string -> Value)
-           (ctxt_fn: string -> list Value -> Value)
-           (ctxt_pred: string -> list Value -> Prop),
-      @formula_semantics Value ctxt_var ctxt_fn ctxt_pred (concl thm).
-
+  Parameter concl: Thm -> formula.
+           
   (*  if |- p ==> q and |- p then |- q                                         *)
   Parameter modus_ponens: Thm -> Thm -> Thm.
 
@@ -434,19 +855,19 @@ Module Type ProofSystem.
   Parameter gen: string -> Thm -> Thm.
   
   (*  |- p ==> (q ==> p)                                                       *)
-  Parameter axiom_addimp: @formula fol -> @formula fol -> Thm.
+  Parameter axiom_addimp: formula -> formula -> Thm.
   
   (*  |- (p ==> q ==> r) ==> (p ==> q) ==> (p ==> r)                           *)
-  Parameter axiom_distribimp: @formula fol -> @formula fol -> @formula fol -> Thm.
+  Parameter axiom_distribimp: formula -> formula -> formula -> Thm.
   
   (*  |- ((p ==> false) ==> false) ==> p                                       *)
-  Parameter axiom_doubleneg: @formula fol -> Thm.
+  Parameter axiom_doubleneg: formula -> Thm.
   
   (*  |- (forall x. p ==> q) ==> (forall x. p) ==> (forall x. q)               *)
-  Parameter axiom_allimp: string -> @formula fol -> @formula fol -> Thm.
+  Parameter axiom_allimp: string -> formula -> formula -> Thm.
     
   (*  |- p ==> forall x. p                            [x not free in p]        *)
-  Parameter axiom_impall: string -> @formula fol -> Thm.
+  Parameter axiom_impall: string -> formula -> Thm.
   
   (*  |- exists x. x = t                              [x not free in t]        *)
   Parameter axiom_existseq: string -> term -> Thm.
@@ -461,436 +882,162 @@ Module Type ProofSystem.
   Parameter axiom_predcong: string -> list term -> list term -> Thm.
   
   (*  |- (p <=> q) ==> p ==> q                                                 *)
-  Parameter axiom_iffimp1: @formula fol -> @formula fol -> Thm.
+  Parameter axiom_iffimp1: formula -> formula -> Thm.
   
   (*  |- (p <=> q) ==> q ==> p                                                 *)
-  Parameter axiom_iffimp2: @formula fol -> @formula fol -> Thm.
+  Parameter axiom_iffimp2: formula -> formula -> Thm.
 
   (*  |- (p ==> q) ==> (q ==> p) ==> (p <=> q)                                 *)
-  Parameter axiom_impiff: @formula fol -> @formula fol -> Thm.
+  Parameter axiom_impiff: formula -> formula -> Thm.
 
   (*  |- true <=> (false ==> false)                                            *)
   Parameter axiom_true: Thm.
   
   (*  |- ~p <=> (p ==> false)                                                  *)
-  Parameter axiom_not: @formula fol -> Thm.
+  Parameter axiom_not: formula -> Thm.
   
   (*  |- p /\ q <=> (p ==> q ==> false) ==> false                              *)
-  Parameter axiom_and: @formula fol -> @formula fol -> Thm.
+  Parameter axiom_and: formula -> formula -> Thm.
   
   (*  |- p \/ q <=> ~(~p /\ ~q)                                                *)
-  Parameter axiom_or: @formula fol -> @formula fol -> Thm.
+  Parameter axiom_or: formula -> formula -> Thm.
 
   (*  |- (exists x. p) <=> ~(forall x. ~p)                                     *)
-  Parameter axiom_exists: string -> @formula fol -> Thm.
+  Parameter axiom_exists: string -> formula -> Thm.
 
 End ProofSystem.
 
 Module Proven: ProofSystem.
 
-  Record Impl: Set := mkImpl {
-                       concl :> formula;
-                       proof: forall 
-                           {Value: InhabitedType}
-                           (ctxt_var: string -> Value)
-                           (ctxt_fn: string -> list Value -> Value)
-                           (ctxt_pred: string -> list Value -> Prop),
-                           formula_semantics ctxt_var ctxt_fn ctxt_pred concl;
-                       }.
+  Definition Thm := { f: formula | |- f }.
 
-  Definition Thm := Impl.
+  Print exist.
 
-  Program Definition T_Thm := mkImpl True _.
+  Check exist.
+  
+  Definition concl (thm: Thm): formula :=
+    match thm with
+    | exist _ x _ => x
+    end.
+
+  Definition prf (thm: Thm): |- concl thm :=
+    match thm with
+    | exist _ _ p => p
+    end.
+  
+  Program Definition T_Thm := exist is_valid true _.
+  Next Obligation.
+    sauto.
+  Qed.
+
+  Definition mkThm f prf: Thm := exist is_valid f prf .
   
   (*  if |- p ==> q and |- p then |- q                                         *)
   Program Definition modus_ponens (thm1 thm2: Thm): Thm :=
     match concl thm1 with
     | Imp f1 f2 =>
       match formula_dec f1 thm2 with
-      | left _ => mkImpl f2 _
+      | left _ => (**) mkThm f2 _
       | right _ => T_Thm
       end
     | _ => T_Thm
     end.
   Next Obligation.
-    generalize (@proof thm1 Value ctxt_var ctxt_fn ctxt_pred); intros.
-    generalize (@proof thm2 Value ctxt_var ctxt_fn ctxt_pred); intros.
-    rewrite <- Heq_anonymous0 in H.
-    simpl in H.
-    intuition.
+    destruct thm1; destruct thm2.
+    eapply modusponens.
+    simpl in Heq_anonymous0.
+    subst x.
+    apply i.
+    apply i0.
   Qed.
     
   (*  if |- p then |- forall x. p                                              *)
-  Program Definition gen (x: string) (thm: Thm): Thm := mkImpl (Forall x thm) _.
-  Next Obligation.
-    apply (@proof thm Value).
-  Qed.
+  Program Definition gen (x: string) (thm: Thm): Thm := mkThm _ (lemma_gen (prf thm) x).
   
   (*  |- p ==> (q ==> p)                                                       *)
-  Program Definition axiom_addimp (p q: formula): Thm := mkImpl (Imp p (Imp q p)) _.
+  Program Definition axiom_addimp (p q: formula): Thm := mkThm _ (lemma_addimp p q).
     
   (*  |- (p ==> q ==> r) ==> (p ==> q) ==> (p ==> r)                           *)
   Program Definition axiom_distribimp (p q r: formula): Thm :=
-    mkImpl (Imp (Imp p (Imp q r)) (Imp (Imp p q) (Imp p r))) _.
+    mkThm _ (lemma_distribimp p q r).
   
   (*  |- ((p ==> false) ==> false) ==> p                                       *)
-  Program Definition axiom_doubleneg (p: formula): Thm := mkImpl (Imp (Imp (Imp p False) False) p) _.
-  Next Obligation.
-    generalize (classical_formula ctxt_var ctxt_fn ctxt_pred p); intro H0; inversion_clear H0; auto.
-    intuition.
-  Qed.  
+  Program Definition axiom_doubleneg (p: formula): Thm :=
+    mkThm _ (lemma_doubleneg p).
   
   (*  |- (forall x. p ==> q) ==> (forall x. p) ==> (forall x. q)               *)
   Program Definition axiom_allimp (x: string) (p q: formula): Thm :=
-    mkImpl (Imp
-              (Forall x (Imp p q))
-              (Imp
-                 (Forall x p)
-                 (Forall x q)
-              )
-        ) _.
+    mkThm _ (lemma_allimp x p q).
     
   (*  |- p ==> forall x. p                            [x not free in p]        *)
   Program Definition axiom_impall (x: string) (p: formula): Thm :=
     match List.in_dec string_dec x (formula_free_vars p) with
     | left _ => T_Thm
-    | right _ => mkImpl (Imp p (Forall x p)) _
+    | right _ => mkThm _ (lemma_impall x p _)
     end.
-  Next Obligation.
-    rewrite formula_semantics_free_vars.
-    apply H.
-    intros.
-    destruct (string_dec x s); auto.
-    subst s; contradiction.
-  Qed.
-  
+   
+                                                                     
   (*  |- exists x. x = t                              [x not free in t]        *)
   Program Definition axiom_existseq (x: string) (t: term) : Thm :=
     match List.in_dec string_dec x (term_free_vars t) with
     | left _ => T_Thm
-    | right _ => mkImpl (Exists x (Eq (var x) t)) _
+    | right _ => mkThm _ (lemma_existseq x t _)
     end.
-  Next Obligation.
-    exists (term_semantics ctxt_var ctxt_fn t).
-    rewrite term_semantics_var.
-    destruct (string_dec x x); [ idtac | intuition ].
-    eapply term_semantics_free_vars; intros.
-    destruct (string_dec x s).
-    subst s; contradiction.
-    auto.
-  Qed.
-
+  
   (*  |- t = t                                                                 *)
-  Program Definition axiom_eqrefl (t: term): Thm := mkImpl (Eq t t) _.    
+  Program Definition axiom_eqrefl (t: term): Thm :=
+    mkThm _ (lemma_eqrefl t).    
   
   (*  |- s1 = t1 ==> ... ==> sn = tn ==> f(s1,..,sn) = f(t1,..,tn)             *)
-  Fixpoint list_term_prefix (l1 l2: list term): list term :=
-    match l2 with
-    | nil  => l1
-    | hd2::tl2 =>
-      match l1 with
-      | nil => nil
-      | hd1::tl1 =>
-        hd2::(list_term_prefix tl1 tl2)
-      end
+  Fixpoint zip (l1 l2: list term): list (term * term) :=
+    match l1 with
+    | nil => nil
+    | hd1::tl1 =>
+        match l2 with
+        | nil => nil
+        | hd2::tl2 => (hd1, hd2)::(zip tl1 tl2)
+        end
     end.
-
-  Lemma list_term_prefix_nil_right: forall l,
-      list_term_prefix l nil = l.
-    induction l; simpl; auto.
-  Qed.
-
-  Fixpoint zip_list_term (l1 l2: list term): list (term * term) :=
-    match l1, l2 with
-    | hd1::tl1, hd2::tl2 =>
-      (hd1, hd2)::(zip_list_term tl1 tl2)
-    | _, _ => nil
-    end.
-
-  Lemma zip_list_term_nil_left: forall l,
-      zip_list_term nil l = nil.
-    intuition.
-  Qed.
-
-  Lemma zip_list_term_nil_right: forall l,
-      zip_list_term l nil = nil.
-    induction l; simpl; intuition.
-  Qed.
-
-  Lemma list_term_semantics_eq_term:
-    forall {Value: InhabitedType}
-           (ctxt_var: string -> Value)
-           (ctxt_fn: string -> list Value -> Value),
-    forall rhs lhs,
-             (forall x, List.In x (zip_list_term lhs rhs) ->
-                        let (x1, x2) := x in
-                        @term_semantics Value ctxt_var ctxt_fn x1 = @term_semantics Value ctxt_var ctxt_fn x2) ->
-             map (@term_semantics Value ctxt_var ctxt_fn) lhs =
-             map (@term_semantics Value ctxt_var ctxt_fn) (list_term_prefix lhs rhs).
-    do 4 intro.
-    induction rhs; simpl; intros; auto.
-    rewrite list_term_prefix_nil_right; auto.
-    destruct lhs; auto.
-    simpl; simpl in H; rewrite (H (t, a)).
-    apply f_equal.
-    apply IHrhs.
-    intros.
-    apply H.
-    right; auto.
-    left; auto.
-Qed.
-
-  Lemma fun_congruence_eq_term:
-    forall {Value: InhabitedType}
-           (ctxt_var: string -> Value)
-           (ctxt_fn: string -> list Value -> Value)
-           (ctxt_pred: string -> list Value -> Prop),
-    forall f rhs lhs,
-             (forall x, List.In x (zip_list_term lhs rhs) ->
-                        let (x1, x2) := x in
-                        @formula_semantics Value ctxt_var ctxt_fn ctxt_pred (Eq x1 x2)
-                        ) ->
-             @formula_semantics Value ctxt_var ctxt_fn ctxt_pred (Eq (fn f lhs) (fn f (list_term_prefix lhs rhs))).
-    simpl; intros.
-    do 2 rewrite term_semantics_fn.
-    rewrite <- list_term_semantics_eq_term; auto.
-  Qed.
-
-  Lemma pred_congruence_eq_term:
-    forall {Value: InhabitedType}
-           (ctxt_var: string -> Value)
-           (ctxt_fn: string -> list Value -> Value)
-           (ctxt_pred: string -> list Value -> Prop),
-    forall P rhs lhs,
-             (forall x, List.In x (zip_list_term lhs rhs) ->
-                        let (x1, x2) := x in
-                        @formula_semantics Value ctxt_var ctxt_fn ctxt_pred (Eq x1 x2)
-                        ) ->
-             @formula_semantics Value ctxt_var ctxt_fn ctxt_pred (
-                                  Imp
-                                    (Atom (R P lhs))
-                                    (Atom (R P (list_term_prefix lhs rhs)))
-                                ).
-    simpl; intros.
-    rewrite <- list_term_semantics_eq_term; auto.
-  Qed.
   
-  Fixpoint build_conj (fs: list (@formula fol)) : formula :=
-    match fs with
-    | nil => True
-    | hd::tl => And hd (build_conj tl)
-    end.
-
-  Lemma build_conj_sem:
-    forall {Value: InhabitedType}
-           (ctxt_var: string -> Value)
-           (ctxt_fn: string -> list Value -> Value)
-           (ctxt_pred: string -> list Value -> Prop),
-    forall l,
-      @formula_semantics Value ctxt_var ctxt_fn ctxt_pred (
-                           build_conj (List.map (fun x: (term * term) => let (x1, x2) := x in Eq x1 x2) l)
-                         ) <->
-      (forall x, List.In x l ->
-                        let (x1, x2) := x in
-                        @formula_semantics Value ctxt_var ctxt_fn ctxt_pred (Eq x1 x2)
-                        ).
-    do 4 intro.
-    induction l; simpl; intros.
-    intuition.
-    split; intros.
-    inversion_clear H.
-    inversion_clear H0.
-    subst a.
-    destruct x.
-    intuition.
-    rewrite IHl in H2.
-    generalize (H2 x H).
-    destruct x; intuition.
-    split.
-    generalize (H a); intros.
-    destruct a.
-    intuition.
-    rewrite IHl.
-    intros.
-    generalize (H x).
-    destruct x; intuition.
-Qed.
-
-  Fixpoint build_imp (fs: list (@formula fol)) (ccl: formula): formula :=
-    match fs with
-    | nil => ccl
-    |hd::tl => Imp hd (build_imp tl ccl)
-    end.
-
-  Lemma build_conj_imp_equiv:
-    forall {Value: InhabitedType}
-           (ctxt_var: string -> Value)
-           (ctxt_fn: string -> list Value -> Value)
-           (ctxt_pred: string -> list Value -> Prop),
-    forall fs ccl,
-      @formula_semantics Value ctxt_var ctxt_fn ctxt_pred (
-                           Imp (build_conj fs) ccl
-                         ) <->
-      @formula_semantics Value ctxt_var ctxt_fn ctxt_pred (
-                           build_imp fs ccl
-                         ).
-    do 4 intro; induction fs; split; simpl; intros.
-    intuition.
-    intuition.
-    rewrite <- IHfs; simpl; intuition.
-    simpl in IHfs.
-    inversion_clear H0.
-    generalize (H H1); intros.
-    rewrite <- IHfs in H0; intros.
-    intuition.
-  Qed.    
-
-  Program Definition axiom_funcong_aux (f: string) (lhs rhs: list term) : Thm :=
-    mkImpl (
-        Imp
-          (build_conj (List.map (fun x: (term * term) => let (x1, x2) := x in Eq x1 x2) (zip_list_term lhs rhs)))
-          (Eq (fn f lhs) (fn f (list_term_prefix lhs rhs)))
-      ) _.
-  Next Obligation.
-    apply (fun_congruence_eq_term ctxt_var ctxt_fn ctxt_pred).
-    rewrite <- build_conj_sem; auto.
-  Qed.
-
   Program Definition axiom_funcong (f: string) (lhs rhs: list term) : Thm :=
-    mkImpl (
-        build_imp
-          (List.map (fun x: (term * term) => let (x1, x2) := x in Eq x1 x2) (zip_list_term lhs rhs))
-          (Eq (fn f lhs) (fn f (list_term_prefix lhs rhs)))
-      ) _.
-  Next Obligation.
-    rewrite <- build_conj_imp_equiv.
-    apply axiom_funcong_aux_obligation_1.
-  Qed.
-  
+    mkThm _ (lemma_funcong f (zip lhs rhs)).
+    
   (*  |- s1 = t1 ==> ... ==> sn = tn ==> P(s1,..,sn) ==> P(t1,..,tn)           *)
-  Program Definition axiom_predcong_aux (P: string) (lhs rhs: list term) : Thm :=
-    mkImpl (
-        Imp
-          (build_conj (List.map (fun x: (term * term) => let (x1, x2) := x in Eq x1 x2) (zip_list_term lhs rhs)))
-          (Imp (Atom (R P lhs)) (Atom (R P (list_term_prefix lhs rhs))))
-      ) _.
-  Next Obligation.
-    apply (pred_congruence_eq_term ctxt_var ctxt_fn ctxt_pred).
-    rewrite <- build_conj_sem; auto.
-    auto.
-  Qed.
-
   Program Definition axiom_predcong (P: string) (lhs rhs: list term) : Thm :=
-    mkImpl (
-        build_imp (List.map (fun x: (term * term) => let (x1, x2) := x in Eq x1 x2) (zip_list_term lhs rhs))
-           (Imp (Atom (R P lhs)) (Atom (R P (list_term_prefix lhs rhs))))
-      ) _.
-  Next Obligation.
-    rewrite <- build_conj_imp_equiv.
-    apply axiom_predcong_aux_obligation_1.
-  Qed.
-  
+    mkThm _ (lemma_predcong P (zip lhs rhs)).
+    
   (*  |- (p <=> q) ==> p ==> q                                                 *)
   Program Definition  axiom_iffimp1 (p q: formula) : Thm :=
-    mkImpl (
-        Imp
-          (Iff p q)
-          (Imp p q)
-        ) _.
-  Next Obligation.
-    rewrite <- H; auto.
-  Qed.
+    mkThm _ (lemma_iffimp1 p q).
   
   (*  |- (p <=> q) ==> q ==> p                                                 *)
   Program Definition axiom_iffimp2 (p q: formula) : Thm :=
-    mkImpl (
-        Imp
-          (Iff p q)
-          (Imp q p)
-        ) _.
-  Next Obligation.
-    rewrite H; auto.
-  Qed.
-
+    mkThm _ (lemma_iffimp2 p q).
+    
   (*  |- (p ==> q) ==> (q ==> p) ==> (p <=> q)                                 *)
   Program Definition axiom_impiff (p q: formula) : Thm :=
-    mkImpl (
-        Imp
-          (Imp p q)
-          (Imp
-             (Imp q p)
-             (Iff p q)
-          )
-        ) _.
-  Next Obligation.
-    split; auto.
-  Qed.
+    mkThm _ (lemma_impiff p q).
   
   (*  |- true <=> (false ==> false)                                            *)
-  Program Definition axiom_true: Thm := mkImpl (Iff True (Imp False False)) _.
-  Next Obligation.
-    split; auto.
-  Qed.
+  Program Definition axiom_true: Thm :=
+    mkThm _ lemma_true.
   
   (*  |- ~p <=> (p ==> false)                                                  *)
-  Program Definition axiom_not (p: formula): Thm := mkImpl (Iff (Not p) (Imp p False)) _.
-  Next Obligation.
-    split; auto.
-  Qed.  
+  Program Definition axiom_not (p: formula): Thm := 
+    mkThm _ (lemma_not p).
   
   (*  |- p /\ q <=> (p ==> q ==> false) ==> false                              *)
   Program Definition axiom_and (p q: formula): Thm :=
-    mkImpl (
-        Iff
-          (And p q)
-          (Imp (Imp p (Imp q False)) False)
-      ) _.
-  Next Obligation.
-    split; intros; auto.
-    intuition.
-    generalize (classical_formula ctxt_var ctxt_fn ctxt_pred p); intro H1.
-    generalize (classical_formula ctxt_var ctxt_fn ctxt_pred q); intro H2.
-    intuition.
-  Qed.
-        
+    mkThm _ (lemma_and p q).
+
   (*  |- p \/ q <=> ~(~p /\ ~q)                                                *)
-  Program Definition axiom_or (p q: formula): Thm :=
-    mkImpl (
-        Iff
-          (Or p q)
-          (Not (And (Not p) (Not q)))
-        ) _.
-  Next Obligation.
-    split; intros; auto.
-    intuition.
-    generalize (classical_formula ctxt_var ctxt_fn ctxt_pred p); intro H1.
-    generalize (classical_formula ctxt_var ctxt_fn ctxt_pred q); intro H2.
-    intuition.
-  Qed.
-
+  Program Definition axiom_or (p q: formula): Thm := 
+    mkThm _ (lemma_or p q).
+  
   (*  |- (exists x. p) <=> ~(forall x. ~p)                                     *)
-  Program Definition axiom_exists (x: string) (p: formula): Thm :=
-    mkImpl (
-        Iff
-          (Exists x p)
-          (Not (Forall x (Not p)))
-        ) _.
-  Next Obligation.
-    split; intros; auto; intros.
-    red; intros.
-    inversion_clear H.
-    generalize (H0 x0).
-    contradiction.
-    generalize (classical_formula ctxt_var ctxt_fn ctxt_pred (Exists x p)); simpl; intro H1.
-    inversion_clear H1; auto.
-    assert Logic.False.
-    apply H.
-    intros; red; intros.
-    apply H0.
-    exists v; auto.
-    intuition.    
-  Qed.
-
+  Program Definition axiom_exists (x: string) (p: formula): Thm := 
+    mkThm _ (lemma_exists x p).
+  
 End Proven.
 
 
@@ -900,9 +1047,306 @@ Require Import ExtrOcamlNatBigInt.
 
 Extraction "harrison.ml" Proven.
 
-
-
-
-
-
+(**  **)
+Lemma imp_refl p: |- p ==> p.
+  generalize (lemma_distribimp p (p ==> p) p); intros.
+  generalize (lemma_addimp p (p ==> p)); intros.
+  generalize (modusponens H H0); intros.
+  generalize (lemma_addimp p p); intros.
+  apply (modusponens H1 H2).
+Qed.  
   
+Lemma imp_undiplicate {p q} (H: |- p ==> p ==> q): |- p ==> q.
+  generalize (lemma_distribimp p p q); intros.
+  generalize (modusponens H0 H); intros.
+  generalize (imp_refl p); intros.
+  apply (modusponens H1 H2).
+Qed.
+
+Lemma add_assum p {q} (H: |- q): |- p ==> q.
+  generalize (lemma_addimp q p); intros.
+  apply (modusponens H0 H).
+Qed.
+
+Lemma imp_add_assum p {q r} (H: |- q ==> r): |- (p ==> q) ==> (p ==> r).
+  generalize (lemma_distribimp p q r); intros.
+  generalize (add_assum p H); intros.
+  apply (modusponens H0 H1).
+Qed.
+
+Lemma imp_trans {p q r} (H0: |- p ==> q) (H1: |- q ==> r): |- p ==> r.
+  apply (modusponens
+           (imp_add_assum p H1)
+           H0
+        ).
+Qed.
+
+Lemma imp_insert q {p r} (H: |- p ==> r): |- p ==> q ==> r.
+  generalize (lemma_addimp r q); intros.
+  apply (imp_trans H H0).
+Qed.
+
+Lemma imp_swap {p q r} (H: |- p ==> q ==> r): |- q ==> p ==> r.
+  generalize (lemma_addimp q p); intro H0.
+  generalize (lemma_distribimp p q r); intro H1.
+  generalize (modusponens H1 H); intro H2.
+  apply (imp_trans H0 H2).
+Qed.
+
+Lemma imp_trans_th p q r: |- (q ==> r) ==> (p ==> q) ==> (p ==> r).
+  apply ( imp_trans
+            (lemma_addimp (q ==> r) p)
+            (lemma_distribimp p q r)
+        ).
+Qed.
+
+Lemma imp_add_concl r {p q} (H: |- p ==> q): |- (q ==> r) ==> (p ==> r).
+  apply (
+      modusponens
+        (imp_swap (imp_trans_th p q r))
+        H
+    ).
+Qed.
+
+Lemma imp_swap_th p q r: |- (p ==> q ==> r) ==> (q ==> p ==> r).
+  apply ( imp_trans
+            (lemma_distribimp p q r)
+            (imp_add_concl
+               (p ==> r)
+               (lemma_addimp q p)
+            )
+        ).
+Qed.
+
+Lemma imp_swap2 {p q r s t u} (H: |- (p ==> q ==> r) ==> (s ==> t ==> u)): |- (q ==> p ==> r) ==> (t ==> s ==> u).
+  apply (
+      imp_trans
+        (imp_swap_th q p r)
+        (imp_trans H (imp_swap_th s t u))
+    ).
+Qed.
+
+Lemma right_mp {p q r} (H0: |- p ==> q ==> r) (H1: |- p ==> q): |- p ==> r.
+  apply (imp_undiplicate (imp_trans H1 (imp_swap H0))).
+Qed.
+
+Lemma iff_imp1 {p q} (H: |- p <=> q): |- p ==> q.
+  generalize (lemma_iffimp1 p q); intros.
+  apply (modusponens H0 H).
+Qed.
+
+Lemma iff_imp2 {p q} (H: |- p <=> q): |- q ==> p.
+  generalize (lemma_iffimp2 p q); intros.
+  apply (modusponens H0 H).
+Qed.
+
+Lemma imp_antisym {p q} (H0: |- p ==> q) (H1: |- q ==> p): |- p <=> q.
+  apply (modusponens
+           (modusponens
+              (lemma_impiff p q)
+              H0
+           )
+           H1
+        ).
+Qed.
+
+Lemma right_doubleneg {p q} (H: |- p ==> (q ==> false) ==> false ): |- p ==> q.
+  generalize (lemma_doubleneg q); intro.
+  generalize (imp_trans H H0); intro.
+  apply H1.
+Qed.
+
+Lemma ex_falso p: |- false ==> p.
+  apply (right_doubleneg
+           (lemma_addimp false (p ==> false))
+        ).
+Qed.
+
+Lemma imp_trans2 {p q r s} (H0: |- p ==> q ==> r) (H1: |- r ==> s): |- p ==> q ==> s.
+  generalize (
+      imp_add_assum p
+        (modusponens
+           (imp_trans_th q r s)
+           H1
+        )
+    ); intro.
+  apply (modusponens H H0).
+Qed.
+
+Lemma truth: |- true.
+  apply (modusponens
+           (iff_imp2 lemma_true)
+           (imp_refl false)
+        ).
+Qed.
+
+Inductive tuple: forall (l: list Prop), Type :=
+| tnil: tuple nil
+| tcons: forall {hd: Prop} (thd: hd) {tl: list Prop} (ttl: tuple tl), tuple (hd::tl).
+
+Lemma tuple_formulas_conj: forall
+    (l: list formula)
+    (t: tuple (map (fun x => |- x) l)),
+    |- formulas_conj l.
+  induction l; simpl; intros; auto.
+  apply truth.
+  inversion_clear t.
+  red; intros.
+  split.
+  apply thd.
+  intuition.
+Qed.
+
+Lemma in_f_map:
+  forall {A B: Type} (f: A -> B) (l: list A) (x: A),
+    In x l ->
+    In (f x) (map f l).
+  induction l.
+  sauto.
+  sauto.
+Qed.
+
+(* interesting *)
+Lemma imp_trans_chain_aux :
+  forall (l: list formula)
+         {p} (Hs: tuple (map (fun x => is_valid x) (map (fun x => p ==> x) l)))
+         {r} (H: |- formulas_conj l ==> r),
+    |- p ==> r.
+  intros.  
+  
+  cut (|- p ==> formulas_conj l).
+  intros.
+  apply (imp_trans H0 H).
+  
+  generalize (tuple_formulas_conj _ Hs); intros.
+
+  red; intros.
+  intro.
+  generalize (H0 _ m); intros.
+  rewrite <- conj_forall_eq_m in H2.
+  rewrite <- (@conj_forall_eq_m l _ m).
+  intros.
+  generalize (H2 (p ==>x) ); intros.
+  apply H4; auto.
+  apply in_f_map; auto.
+Qed.
+
+Lemma imp_trans_chain :
+  forall (l: list formula)
+         {p} (Hs: tuple (map (fun x => is_valid x) (map (fun x => p ==> x) l)))
+         {r} (H: |- formulas_imp l r),
+    |- p ==> r.
+  intros.
+  eapply imp_trans_chain_aux.
+  apply Hs.
+  red; intros.
+  generalize (H _ m); intros.
+  rewrite build_conj_imp_equiv.
+  auto.
+Qed.
+
+Lemma imp_truefalse p q: |- (q ==> false) ==> p ==> (p ==> q) ==> false.
+  apply ( imp_trans
+            (imp_trans_th p q false)
+            (imp_swap_th
+               (p ==> q)
+               p
+               false
+            )
+        ).
+Qed.
+
+Lemma imp_mono p p' q q': |- (p' ==> p) ==> (q ==> q') ==> (p ==> q) ==> p' ==> q'.
+  generalize (imp_trans_th (p ==> q) (p' ==> q) (p' ==> q')); intro H1.
+  generalize (imp_trans_th p' q q'); intro H2.
+  generalize (imp_swap (imp_trans_th p' p q)); intro H3.
+  apply (imp_trans H3 (imp_swap (imp_trans H2 H1))).
+Qed.
+
+
+Lemma contrapos {p q} (H: |- p ==> q): |- ~~ q ==> ~~ p.
+  apply (imp_trans
+           (imp_trans
+              (iff_imp1 (lemma_not q))
+              (imp_add_concl false H)
+           )
+           (iff_imp2 (lemma_not p))
+    ).
+Qed.
+
+Lemma and_left p q: |- p //\\ q ==> p.
+  generalize (imp_add_assum p (lemma_addimp false q)); intro H1.
+  generalize (right_doubleneg (imp_add_concl false H1)); intro H2.
+  apply (imp_trans (iff_imp1 (lemma_and p q)) H2).
+Qed.
+
+Lemma and_right p q: |- p //\\ q ==> q.
+  generalize (lemma_addimp (q ==> false) p); intro H1.
+  generalize (right_doubleneg (imp_add_concl false H1)); intro H2.
+  apply (imp_trans
+           (iff_imp1 (lemma_and p q))
+           H2
+        ).
+Qed.
+
+
+(*
+Lemma conjths
+ *)
+
+Lemma and_pair p q: |- p ==> q ==> p //\\ q.
+  generalize (iff_imp2 (lemma_and p q)); intro H1.
+  generalize (imp_swap_th (p ==> q ==> false) q false); intro H2.
+  generalize (imp_add_assum p (imp_trans2 H2 H1)); intro H3.
+  apply (modusponens
+           H3
+           (imp_swap (imp_refl (p ==> q ==> false)))
+        ).
+Qed.
+
+Lemma shunt {p q r} (H: |- p //\\ q ==> r): |- p ==> q ==> r.
+  generalize (fold_right); intro.
+  apply (modusponens
+           (imp_add_assum p (imp_add_assum q H))
+           (and_pair p q)
+        ).
+Qed.
+
+Lemma unshut {p q r} (H: |- p ==> q ==> r): |- p //\\ q ==> r.
+  
+  generalize (tcons (and_left p q) (tcons (and_right p q) tnil)); intro.
+  
+  apply (@imp_trans_chain [p; q] (p //\\ q)); intros.
+
+  eapply tcons.
+  apply and_left.
+  eapply tcons.
+  apply and_right.
+  apply tnil.
+
+  auto.
+Qed.
+
+(******)
+
+(* p. 506 => tableau procedure ~~> Elpi*)
+
+(*** interactive proof style ***)
+
+Record goal: Type := {
+    hypothesises: list formula;
+    ccl: formula;
+    justification: |- formulas_conj hypothesises ==> ccl
+  }.
+
+Lemma close_goal (g: goal) (t: tuple (map (fun x => |- x) (hypothesises g) )): |- ccl g.
+  destruct g.
+  simpl in t; simpl.
+  generalize (tuple_formulas_conj _ t); intros.
+  apply (modusponens justification0 H).
+Qed.
+
+(*
+Definition update_goals
+             (root: goal)
+*)
